Remove install oracle from backend/proofs

compiler/backend/proofs/lab_filterProofScript.sml
@@ -177,14 +177,9 @@ val all_skips_evaluate = Q.prove(`
     metis_tac[arithmeticTheory.ADD_COMM,ADD_ASSOC])
 
 val state_rel_def = Define `
-  state_rel (s1:('a,'c,'ffi) labSem$state) t1 ⇔
-    (∃s1compile.
-     s1 = t1 with <| code := filter_skip t1.code ;
-                     pc := adjust_pc t1.pc t1.code ;
-                     compile_oracle := λn. (λ(a,b).(a,filter_skip b)) (t1.compile_oracle n);
-                     compile := s1compile
-                     |> ∧
-    t1.compile = λc p. s1compile c (filter_skip p)  ) ∧
+  state_rel (s1:('a,'ffi) labSem$state) t1 ⇔
+    (s1 = t1 with <| code := filter_skip t1.code ;
+                     pc := adjust_pc t1.pc t1.code |>) ∧
     ¬t1.failed`
 
 val adjust_pc_all_skips = Q.prove(`
@@ -520,7 +515,7 @@ val upd_pc_tac =
   metis_tac[arithmeticTheory.ADD_COMM,arithmeticTheory.ADD_ASSOC];
 
 val filter_correct = Q.store_thm("filter_correct",
-  `!(s1:('a,'c,'ffi) labSem$state) t1 res s2.
+  `!(s1:('a,'ffi) labSem$state) t1 res s2.
       (evaluate s1 = (res,s2)) /\ state_rel s1 t1 /\ ~t1.failed ==>
       ?k t2.
         (evaluate (t1 with clock := s1.clock + k) = (res,t2)) /\
@@ -552,7 +547,7 @@ val filter_correct = Q.store_thm("filter_correct",
         (rw[]>>
         fs[inc_pc_def,dec_clock_def]>>
         qmatch_asmsub_abbrev_tac`evaluate tt = (res,s2)`>>
-        first_x_assum(qspec_then `tt with <|pc:= t1.pc+k+1; code:=t1.code; compile:= t1.compile; compile_oracle := t1.compile_oracle|>` mp_tac)>>
+        first_x_assum(qspec_then `tt with <|pc:= t1.pc+k+1; code:=t1.code |>` mp_tac)>>
         simp[Abbr`tt`,state_component_equality]>>
         impl_tac>-
           metis_tac[adjust_pc_all_skips,ADD_COMM,ADD_ASSOC]>>
@@ -576,7 +571,7 @@ val filter_correct = Q.store_thm("filter_correct",
           qexists_tac`k`>>qexists_tac`t1 with pc:=k+t1.pc`>>full_simp_tac(srw_ss())[]>>NO_TAC)>>
         (* normal cases *)
         (qmatch_asmsub_abbrev_tac`evaluate tt = (res,s2)`>>
-        first_x_assum(qspec_then `tt with <|pc:= t1.pc+k+1; code:=t1.code; compile:= t1.compile; compile_oracle := t1.compile_oracle|>` mp_tac)>>
+        first_x_assum(qspec_then `tt with <|pc:= t1.pc+k+1; code:=t1.code |>` mp_tac)>>
         simp[Abbr`tt`,state_component_equality]>>
         impl_tac>-
           metis_tac[adjust_pc_all_skips,ADD_COMM,ADD_ASSOC]>>
@@ -600,7 +595,7 @@ val filter_correct = Q.store_thm("filter_correct",
           qexists_tac`k`>>qexists_tac`t1 with pc:=k+t1.pc`>>full_simp_tac(srw_ss())[]>>NO_TAC)>>
         (* everything else*)
         (qmatch_asmsub_abbrev_tac`evaluate tt = (res,s2)`>>
-        first_x_assum(qspec_then `tt with <|pc:= t1.pc+k+1; code:=t1.code; compile:= t1.compile; compile_oracle := t1.compile_oracle|>` mp_tac)>>
+        first_x_assum(qspec_then `tt with <|pc:= t1.pc+k+1; code:=t1.code |>` mp_tac)>>
         simp[Abbr`tt`,state_component_equality]>>
         impl_tac>-
           metis_tac[adjust_pc_all_skips,ADD_COMM,ADD_ASSOC]>>
@@ -620,26 +615,7 @@ val filter_correct = Q.store_thm("filter_correct",
         imp_res_tac loc_to_pc_eq_SOME>>
         full_simp_tac(srw_ss())[get_pc_value_def,upd_pc_def,dec_clock_def]>>srw_tac[][]>>
         upd_pc_tac)
-    >- (*CBW*)
-      (reverse(simp[case_eq_thms]>>rw[]>>fs[inc_pc_def,dec_clock_def])
-      >> TRY (
-        rename1`code_buffer_write _ _ _ = SOME _`>>
-        qmatch_asmsub_abbrev_tac`evaluate tt = (res,s2)`>>
-        first_x_assum(qspec_then `tt with <|pc:= t1.pc+k+1; code:=t1.code; compile:= t1.compile; compile_oracle := t1.compile_oracle|>` mp_tac)>>
-        simp[Abbr`tt`,state_component_equality]>>
-        impl_tac>-
-          metis_tac[adjust_pc_all_skips,ADD_COMM,ADD_ASSOC]>>
-        strip_tac>>
-        first_x_assum(qspec_then`k'` assume_tac)>>
-        qmatch_asmsub_abbrev_tac`evaluate tt = (res,t2)`>>
-        qmatch_asmsub_abbrev_tac`evaluate ss = evaluate _`>>
-        `ss = tt` by (
-          unabbrev_all_tac>>fs[state_component_equality])>>
-        unabbrev_all_tac>>fs[]>>
-        metis_tac[ADD_ASSOC])
-      >>
-        (first_x_assum(qspec_then`0` (assume_tac o SYM))>>
-        fs[]>>qexists_tac`k`>>fs[])))
+      )
   >>
     Cases_on`a`>>
     full_simp_tac(srw_ss())[asm_fetch_def,state_rel_def]>>rev_full_simp_tac(srw_ss())[]>>
@@ -677,7 +653,7 @@ val filter_correct = Q.store_thm("filter_correct",
         (fs[inc_pc_def,dec_clock_def]>>rw[]>>
         fs[]>>
         qmatch_asmsub_abbrev_tac`evaluate tt = (res,s2)`>>
-        first_x_assum(qspec_then `tt with <|pc:= t1.pc+k+1; code:=t1.code; compile:= t1.compile; compile_oracle := t1.compile_oracle|>` mp_tac)>>
+        first_x_assum(qspec_then `tt with <|pc:= t1.pc+k+1; code:=t1.code |>` mp_tac)>>
         simp[Abbr`tt`,state_component_equality]>>
         impl_tac>-
           metis_tac[adjust_pc_all_skips,ADD_COMM,ADD_ASSOC]>>
@@ -711,7 +687,7 @@ val filter_correct = Q.store_thm("filter_correct",
         >>
           fs[upd_pc_def,dec_clock_def,upd_reg_def]>>rw[]>>fs[]>>
           qmatch_asmsub_abbrev_tac`evaluate tt = (res,s2)`>>
-          first_x_assum(qspec_then `tt with <|pc:= pc'; code:=t1.code; compile:= t1.compile; compile_oracle := t1.compile_oracle|>` mp_tac)>>
+          first_x_assum(qspec_then `tt with <|pc:= pc'; code:=t1.code |>` mp_tac)>>
           simp[Abbr`tt`,state_component_equality]>>
           strip_tac>>
           first_x_assum(qspec_then`k'` assume_tac)>>
@@ -758,58 +734,6 @@ val filter_correct = Q.store_thm("filter_correct",
         imp_res_tac loc_to_pc_eq_SOME>>full_simp_tac(srw_ss())[]>>
         pairarg_tac>>full_simp_tac(srw_ss())[]>>
         srw_tac[][]>>upd_pc_tac)
-    >- (*oracle case *)
-      (reverse(Cases_on`t1.regs t1.ptr_reg`) \\ fs[] >- same_inst_tac \\
-      (Cases_on`t1.regs t1.link_reg`) \\ fs[] >- same_inst_tac \\
-      reverse(Cases_on`t1.regs t1.len_reg`) \\ fs[] >- same_inst_tac \\
-      TOP_CASE_TAC >- same_inst_tac \\
-      strip_tac \\
-      TOP_CASE_TAC >- (
-        fs[loc_to_pc_eq_NONE] \\ rw[]
-        \\ first_x_assum(qspec_then`0`mp_tac) \\ rw[]
-        \\ qexists_tac`k` \\ simp[] ) \\
-      split_pair_case_tac \\ fs[] \\
-      pairarg_tac>>fs[] \\
-      imp_res_tac loc_to_pc_eq_SOME \\ fs[] \\
-      TOP_CASE_TAC >- (
-        rw[]>>pairarg_tac>>fs[]>>
-        Cases_on`b`>>fs[filter_skip_MAP]>>
-        same_inst_tac)>>
-      TOP_CASE_TAC>-(
-        rw[]>>pairarg_tac>>fs[]>>
-        Cases_on`b`>>Cases_on`h`>>fs[filter_skip_MAP]>>
-        same_inst_tac)>>
-      split_pair_case_tac \\ fs[] \\
-      TOP_CASE_TAC >> fs[] >>
-      reverse IF_CASES_TAC >- (
-        rw[]>>pairarg_tac>>fs[]>>
-        Cases_on`b`>>fs[filter_skip_MAP]>>
-        Cases_on`h`>>same_inst_tac>>
-        fs[shift_seq_def]>>
-        pairarg_tac>>fs[])>>
-      strip_tac>>
-      pairarg_tac>>fs[shift_seq_def]>>
-      pairarg_tac>>fs[]>>
-      fs[]>>rfs[]>>
-      rw[]>>
-      first_x_assum(qspec_then `t1 with <|
-        regs := (t1.ptr_reg =+ Loc n'' 0) (λa. get_reg_value (t1.cc_regs 0 a) (read_reg a t1) Word);
-        pc := pc';
-        code := t1.code ++ SND(t1.compile_oracle 0);
-        compile_oracle := shift_seq 1 t1.compile_oracle;
-        code_buffer := cb; clock:=t1.clock-1 ; cc_regs:= shift_seq 1 t1.cc_regs|>` mp_tac)>>
-      simp[state_component_equality]>>
-      impl_tac>- (
-        rw[filter_skip_MAP,shift_seq_def]
-        >-
-          metis_tac[loc_to_pc_adjust_pc_append]
-        >>
-          metis_tac[FUN_EQ_THM,filter_skip_MAP])>>
-      rw[]>>
-      first_x_assum(qspec_then`k''` assume_tac)>>rfs[]>>
-      Cases_on`b`>>fs[filter_skip_MAP]>>
-      Cases_on`h`>>fs[shift_seq_def]>>
-      metis_tac[ADD_ASSOC])
     >>
       EVERY_CASE_TAC>>full_simp_tac(srw_ss())[]>>srw_tac[][]>>
       same_inst_tac);
@@ -928,17 +852,10 @@ val state_rel_IMP_sem_EQ_sem = Q.prove(
     metis_tac[build_lprefix_lub_thm,unique_lprefix_lub,lprefix_lub_new_chain]));
 
 val filter_skip_semantics = Q.store_thm("filter_skip_semantics",
-  `!s t. (t.pc = 0) ∧ ¬t.failed /\
-   (∃scompile.
-     s = t with <| code := filter_skip t.code ;
-                   compile_oracle := (λ(a,b).(a,filter_skip b)) o t.compile_oracle;
-                   compile := scompile
-                 |> ∧
-    t.compile = λc p. scompile c (filter_skip p)) ∧
-    ¬t.failed  ==>
-  semantics s = semantics t`,
+  `!s t. (s.pc = 0) ∧ ¬s.failed /\ (t = s with code := filter_skip s.code) ==>
+          semantics t = semantics s`,
   srw_tac[][] \\ match_mp_tac state_rel_IMP_sem_EQ_sem
-  \\ full_simp_tac(srw_ss())[state_rel_def,state_component_equality,Once adjust_pc_def,o_DEF]);
+  \\ full_simp_tac(srw_ss())[state_rel_def,state_component_equality,Once adjust_pc_def]);
 
 val sec_ends_with_label_filter_skip = Q.store_thm("sec_ends_with_label_filter_skip",
   `∀code.
